base version using built-in canonical forms

src/computational_monads/oracle_comp_base.lean
@@ -9,73 +9,33 @@ import probability.probability_mass_function.basic
 
 universes u v
 
-
--- inductive assoc_equiv {spec : oracle_spec} :
---   Π {α : Type}, oracle_comp_base spec α →
---     oracle_comp_base spec α → Prop
--- | refl {α : Type} (oa : oracle_comp_base spec α) :
---     assoc_equiv oa oa
--- | symm {α : Type} (oa oa' : oracle_comp_base spec α) :
---     assoc_equiv oa oa' → assoc_equiv oa' oa
--- | trans {α : Type} (oa oa' oa'' : oracle_comp_base spec α) :
---     assoc_equiv oa oa' → assoc_equiv oa' oa'' → assoc_equiv oa oa''
--- | bind_assoc {α β γ : Type} (oa : oracle_comp_base spec α)
---     (ob : α → oracle_comp_base spec β) (oc : β → oracle_comp_base spec γ) :
---     assoc_equiv (bind' β γ (bind' α β oa ob) oc)
---       (bind' α γ oa (λ x, bind' β γ (ob x) oc))
-
-inductive is_lawfully_equiv (m : Type u → Type v) [monad m] :
-  Π {α : Type u}, m α → m α → Prop
-| refl {α : Type u} (x : m α) : is_lawfully_equiv x x
-| symm {α : Type u} (x y : m α) (h : is_lawfully_equiv x y) :
-    is_lawfully_equiv y x
-| trans {α : Type u} (x y z : m α) (h : is_lawfully_equiv x y) (h' : is_lawfully_equiv y z) :
-    is_lawfully_equiv x z
-| pure_bind {α β : Type u} (a : α) (y : α → m β) :
-    is_lawfully_equiv (pure a >>= y) (y a)
-| bind_assoc {α β γ : Type u} (x : m α) (y : α → m β) (z : β → m γ) :
-    is_lawfully_equiv ((x >>= y) >>= z) (x >>= λ a, (y a >>= z))
-| map_id {α : Type u} (x : m α) :
-    is_lawfully_equiv (x >>= pure) x
-| bind_congr {α β : Type u} (x x' : m α) (y y' : α → m β)
-    (hx : is_lawfully_equiv x x') (hy : ∀ a, is_lawfully_equiv (y a) (y' a)) :
-    is_lawfully_equiv (x >>= y) (x' >>= y')
-
--- #check is_lawfully_equiv.bind_assoc
--- -- def lawfully_reduce (m : Type u → Type v)
-
-lemma is_lawfully_equiv.equivalence (m : Type u → Type v) [monad m] (α : Type u) :
-  equivalence (@is_lawfully_equiv m _ α) :=
-⟨is_lawfully_equiv.refl, is_lawfully_equiv.symm, is_lawfully_equiv.trans⟩
-
 open oracle_spec
 
-
-inductive oracle_comp' (spec : oracle_spec) : Type → Type 1
-| pure' (α : Type) (a : α) : oracle_comp' α
-| query' (i : spec.ι) (t : spec.domain i) : oracle_comp' (spec.range i)
+inductive oracle_comp_base (spec : oracle_spec) : Type → Type 1
+| pure' (α : Type) (a : α) : oracle_comp_base α
+| query' (i : spec.ι) (t : spec.domain i) : oracle_comp_base (spec.range i)
 | query_bind' (i : spec.ι) (t : spec.domain i) (α : Type)
-    (ou : spec.range i → oracle_comp' α) : oracle_comp' α
+    (ou : spec.range i → oracle_comp_base α) : oracle_comp_base α
 
-section oracle_comp'
+namespace oracle_comp_base
 
-open oracle_comp'
+open oracle_comp_base
 
 def bind' {spec : oracle_spec} : Π (α β : Type),
-  oracle_comp' spec α → (α → oracle_comp' spec β) →
-    oracle_comp' spec β
+  oracle_comp_base spec α → (α → oracle_comp_base spec β) →
+    oracle_comp_base spec β
 | _ β (pure' α a) ob := ob a
 | _ β (query' i t) ob := query_bind' i t β ob
 | _ β (query_bind' i t α ou) ob :=
         query_bind' i t β (λ u, bind' α β (ou u) ob)
 
-lemma pure_bind {spec : oracle_spec} {α β : Type}
-  (a : α) (ob : α → oracle_comp' spec β) :
+lemma pure'_bind' {spec : oracle_spec} {α β : Type}
+  (a : α) (ob : α → oracle_comp_base spec β) :
   bind' α β (pure' α a) ob = ob a := rfl
 
-lemma bind_assoc {spec : oracle_spec} {α β γ : Type}
-  (oa : oracle_comp' spec α) (ob : α → oracle_comp' spec β)
-  (oc : β → oracle_comp' spec γ) :
+lemma bind'_assoc {spec : oracle_spec} {α β γ : Type}
+  (oa : oracle_comp_base spec α) (ob : α → oracle_comp_base spec β)
+  (oc : β → oracle_comp_base spec γ) :
   bind' β γ (bind' α β oa ob) oc =
     bind' α γ oa (λ x, bind' β γ (ob x) oc) :=
 begin
@@ -86,206 +46,69 @@ begin
     refine funext (λ u, h u ob) }
 end
 
-section red
+section reduce
 
 open_locale classical
 
-noncomputable def red {spec : oracle_spec} : Π {α : Type},
-  oracle_comp' spec α → oracle_comp' spec α
+noncomputable def reduce {spec : oracle_spec} : Π {α : Type},
+  oracle_comp_base spec α → oracle_comp_base spec α
 | _ (pure' α a) := pure' α a
 | _ (query' i t) := query' i t
 | _ (query_bind' i t α ou) := begin
   refine (if h : α = spec.range i then _ else _),
   {
     -- induction h,
-    refine if h.rec_on ou = pure' (spec.range i) then
+    refine if h.rec_on (λ u, reduce (ou u)) = pure' (spec.range i) then
       h.symm.rec_on (query' i t) else _,
-    refine query_bind' i t α (λ u, red (ou u)),
+    refine query_bind' i t α (λ u, reduce (ou u)),
   },
-  refine query_bind' i t α (λ u, red (ou u))
+  refine query_bind' i t α (λ u, reduce (ou u))
 end
 
-lemma red_bind_pure {spec : oracle_spec} {α : Type}
-  (oa : oracle_comp' spec α) :
-  red (bind' α α oa (pure' α)) = red oa :=
+-- lemma reduce_bind' {spec : oracle_spec} {α : Type}
+--   (oa : oracle_comp_base spec α) :
+
+@[simp] lemma reduce_idem {spec : oracle_spec} {α : Type}
+  (oa : oracle_comp_base spec α) : oa.reduce.reduce = oa.reduce :=
 begin
   induction oa with α a i t i t α ou h,
-  {
-    simp [red, bind'],
-  },
-  {
-    simp [red, bind'],
-  },
+  { refl },
+  { refl },
   {
     by_cases hα : spec.range i = α,
-    {
-
-      induction hα,
-      simp at h,
-      simp [red, bind', h],
-
-    }
-  }
-end
-
-end red
-
-end oracle_comp'
-
--- instance (spec : oracle_spec) : monad (oracle_comp' spec) :=
--- { pure := oracle_comp'.pure',
---   bind := λ α β oa ob, match oa with
---     | (oracle_comp'.pure' α a) := ob a
---     | (oracle_comp'.query i t) := _
---   end }
-
-
-
-
-
-
-
-
-
-
-
-
-/-- Type to represent computations with access so oracles specified by and `oracle_spec`. -/
-inductive oracle_comp_base (spec : oracle_spec) : Type → Type 1
-| pure' (α : Type) (a : α) : oracle_comp_base α
-| bind' (α β : Type) (oa : oracle_comp_base α) (ob : α → oracle_comp_base β) : oracle_comp_base β
-| query (i : spec.ι) (t : spec.domain i) : oracle_comp_base (spec.range i)
-
-namespace oracle_comp_base
-
-def extract_pure {spec : oracle_spec} :
-  Π {α : Type}, oracle_comp_base spec α → option α
-| _ (pure' α a) := some a
-| _ (bind' α β oa ob) := none
-| _ (query i t) := none
-
-lemma extract_pure_eq_some_iff {spec : oracle_spec} {α : Type}
-  (oa : oracle_comp_base spec α) (a : α) :
-  oa.extract_pure = some a ↔ oa = pure' α a :=
-sorry
-
-section reduce_pure
-
-open_locale classical
-
-
-inductive reduce_result (spec : oracle_spec) (α : Type)
--- Computation was reduced to the form `pure' α a`
-| free_value (a : α) : reduce_result
-| bound_query (i : spec.ι) (t : spec.domain i)
-    (ob : spec.range i → oracle_comp_base spec α) : reduce_result
-| free_computation (oa : oracle_comp_base spec α) : reduce_result
-
-open reduce_result
-
-#check reduce_result.sizeof
-
-#check psigma.lex
-
--- def unreduce {spec : oracle_spec} :
---   Π {α : Type}, reduce_result spec α → oracle_comp_base spec α
--- | α (free_value a) := pure' α a
--- | β (bound_query i t ob) := bind' (spec.range i) β (query i t)
---     (λ u, unreduce (ob u))
-
-
-def reduce_aux' {spec : oracle_spec} :
-  Π {α : Type}, reduce_result spec α →
-    oracle_comp_base spec α → reduce_result spec α
-| _ rr (query i t) := _
-| _ rr (pure' α a) := _
-| _ rr (bind' α β oa ob) := _
-
-def reduce_aux {spec : oracle_spec} :
-  Π {α : Type}, oracle_comp_base spec α → reduce_result spec α
-| _ (query i t) := reduce_result.free_computation (query i t)
-| _ (pure' α a) := reduce_result.free_value a
-| _ (bind' α β oa ob) := let oa' := reduce_aux oa in
-  match oa' with
-  | (free_value a) := reduce_aux (ob a)
-  | (bound_query i t oc) :=
-      bound_query i t (λ u, bind' _ _ (oc u) ob)
-  | (free_computation oa) :=
-      free_computation (bind' α β oa ob)
-
-  end
-
-
-noncomputable def reduce_pure {spec : oracle_spec} :
-  Π {α : Type}, oracle_comp_base spec α → oracle_comp_base spec α
-| _ (pure' α a) := pure' α a
-| _ (bind' α β oa ob) := let oa' := reduce_pure oa in
-  match extract_pure oa' with
-  | (some a) := reduce_pure (ob a)
-  | none := if h : β = α then
-    (if h.rec_on (λ x, reduce_pure (ob x)) = (pure' α) then
-      h.symm.rec oa' else bind' α β oa' (λ x, reduce_pure (ob x)))
-        else bind' α β oa' (λ x, reduce_pure (ob x))
-  end
-| _ (query i t) := query i t
-
-end reduce_pure
-
-section reduce_assoc
-
-noncomputable def reduce_assoc {spec : oracle_spec} :
-  Π {α : Type}, oracle_comp_base spec α → oracle_comp_base spec α
-| _ (pure' α a) := pure' α a
-| _ (bind' _ γ (bind' α β oa ob) oc) := sorry
-| _ (query i t) := query i t
-
-end reduce_assoc
-
-@[simp] lemma reduce_pure_idem {spec : oracle_spec} {α : Type}
-  (oa : oracle_comp_base spec α) : reduce_pure (reduce_pure oa) = reduce_pure oa :=
-begin
-  induction oa with α a α β oa ob hoa hob i t,
-  {
-    simp [reduce_pure],
-  },
-  {
-    simp [reduce_pure],
-    by_cases ha : ∃ a, oa.reduce_pure.extract_pure = some a,
-    {
-      obtain ⟨a, ha⟩ := ha,
-      simp [ha, reduce_pure, hob],
-    },
-    {
-      rw [← option.is_some_iff_exists] at ha,
-      simp [option.is_none_iff_eq_none] at ha,
-      simp [ha, reduce_pure],
-      by_cases h : β = α,
+    { induction hα,
+      simp [reduce],
+      split_ifs with h',
       {
-        induction h,
-        simp,
-        split_ifs with hb,
-        {
-          exact hoa,
-        },
-        {
-          simp [reduce_pure, ha, hoa, hob, hb],
-        }
+        simp [reduce],
       },
       {
-
-        simp [h, reduce_pure, hoa, ha, hob],
+        simp [reduce, h, h'],
       }
-    }
-  },
-  {
-    simp [reduce_pure]
+    },
+    { simp [reduce, bind', ne.symm hα, h],
+
+     }
   }
 end
 
+@[simp] lemma reduce_bind_pure {spec : oracle_spec} {α : Type}
+  (oa : oracle_comp_base spec α) :
+  reduce (bind' α α oa (pure' α)) = reduce oa :=
+begin
+  induction oa with α a i t i t α ou h,
+  { simp [reduce, bind'] },
+  { simp [reduce, bind'] },
+  { by_cases hα : α = spec.range i,
+    { simp [reduce, bind', hα, h] },
+    { simp [reduce, bind', hα, h] } },
+end
+
+end reduce
 
 instance setoid (spec : oracle_spec) (α : Type) :
   setoid (oracle_comp_base spec α) :=
-{ r := λ oa oa', reduce_pure oa = reduce_pure oa',
+{ r := λ oa oa', reduce oa = reduce oa',
   iseqv := ⟨λ _, rfl, λ _ _, eq.symm, λ _ _ _, eq.trans⟩ }
 
 end oracle_comp_base
@@ -295,14 +118,16 @@ quotient (oracle_comp_base.setoid spec α)
 
 namespace oracle_comp
 
+-- open
+
 noncomputable instance monad (spec : oracle_spec) :
   monad (oracle_comp spec) :=
 { pure := λ α a, ⟦oracle_comp_base.pure' α a⟧,
   bind := λ α β oa ob, begin
     refine quotient.lift_on oa (λ oa', ⟦_⟧) (λ oa₁ oa₂ h, _),
     refine oracle_comp_base.bind' α β
-      (oracle_comp_base.reduce_pure oa')
-      (λ x, quotient.lift_on (ob x) oracle_comp_base.reduce_pure
+      (oracle_comp_base.reduce oa')
+      (λ x, quotient.lift_on (ob x) oracle_comp_base.reduce
       (λ ob₁ ob₂ h, h)),
     refine quotient.eq.2 (by congr; exact h),
   end }
@@ -315,118 +140,69 @@ lemma bind_def {spec : oracle_spec} {α β : Type}
   oa >>= ob = begin
 refine quotient.lift_on oa (λ oa', ⟦_⟧) (λ oa₁ oa₂ h, _),
     refine oracle_comp_base.bind' α β
-      (oracle_comp_base.reduce_pure oa')
-      (λ x, quotient.lift_on (ob x) oracle_comp_base.reduce_pure
+      (oracle_comp_base.reduce oa')
+      (λ x, quotient.lift_on (ob x) oracle_comp_base.reduce
       (λ ob₁ ob₂ h, h)),
     refine quotient.eq.2 (by congr; exact h),
-
   end  := rfl
 
 
 instance is_lawful_monad (spec : oracle_spec) :
   is_lawful_monad (oracle_comp spec) :=
 { pure_bind := λ α β a ob, begin
-    simp [bind_def, pure_def, oracle_comp_base.reduce_pure],
+
+    simp [bind_def, pure_def, oracle_comp_base.reduce],
     obtain ⟨ob', h⟩ := quotient.exists_rep (ob a),
     refine trans _ h,
     refine quotient.sound _,
-    show oracle_comp_base.reduce_pure _ = oracle_comp_base.reduce_pure _,
-    simp [oracle_comp_base.reduce_pure,
-      oracle_comp_base.extract_pure, ← h],
+    show oracle_comp_base.reduce _ = oracle_comp_base.reduce _,
+    simp [oracle_comp_base.bind', oracle_comp_base.reduce, ← h],
+    -- simp [oracle_comp_base.reduce, ← h],
   end,
-  bind_assoc := begin
-
+  bind_assoc := λ α β γ oa ob oc, begin
+    simp [bind_def, pure_def, oracle_comp_base.reduce],
+    obtain ⟨oa', h⟩ := quotient.exists_rep oa,
+    simp [← h],
+    show oracle_comp_base.reduce _ = oracle_comp_base.reduce _,
+    sorry,
   end,
   id_map := λ α oa, begin
+
     show oa >>= (λ x, pure x) = oa,
-    simp [bind_def, pure_def, oracle_comp_base.reduce_pure],
+    simp [bind_def, pure_def, oracle_comp_base.reduce],
     obtain ⟨oa', h⟩ := quotient.exists_rep oa,
     simp [← h],
     -- refine quotient.sound _,
-    show oracle_comp_base.reduce_pure _ = oracle_comp_base.reduce_pure _,
-    simp [oracle_comp_base.reduce_pure,
-      oracle_comp_base.extract_pure, ← h],
-    by_cases ha : ∃ a, oa'.reduce_pure.extract_pure = some a,
-    {
-      obtain ⟨a, ha⟩ := ha,
-      simp [ha, oracle_comp_base.reduce_pure],
-      induction oa',
-      {
-        simp [oracle_comp_base.reduce_pure,
-          oracle_comp_base.extract_pure] at ha,
-        simp [ha, oracle_comp_base.reduce_pure]
-      },
-      {
+    show oracle_comp_base.reduce _ = oracle_comp_base.reduce _,
+    simp,
+    -- simp [oracle_comp_base.reduce_pure,
+    --   oracle_comp_base.extract_pure, ← h],
+    -- by_cases ha : ∃ a, oa'.reduce_pure.extract_pure = some a,
+    -- {
+    --   obtain ⟨a, ha⟩ := ha,
+    --   simp [ha, oracle_comp_base.reduce_pure],
+    --   induction oa',
+    --   {
+    --     simp [oracle_comp_base.reduce_pure,
+    --       oracle_comp_base.extract_pure] at ha,
+    --     simp [ha, oracle_comp_base.reduce_pure]
+    --   },
+    --   {
 
-        simp [oracle_comp_base.extract_pure_eq_some_iff] at ha,
-        exact symm ha,
-      },
-      {
-        simp [oracle_comp_base.extract_pure_eq_some_iff,
-          oracle_comp_base.reduce_pure] at ha,
-        exact false.elim ha,
-      }
-    },
-    {
-      rw [← option.is_some_iff_exists] at ha,
-      simp [option.is_none_iff_eq_none] at ha,
-      simp [ha, oracle_comp_base.reduce_pure],
-    }
+    --     simp [oracle_comp_base.extract_pure_eq_some_iff] at ha,
+    --     exact symm ha,
+    --   },
+    --   {
+    --     simp [oracle_comp_base.extract_pure_eq_some_iff,
+    --       oracle_comp_base.reduce_pure] at ha,
+    --     exact false.elim ha,
+    --   }
+    -- },
+    -- {
+    --   rw [← option.is_some_iff_exists] at ha,
+    --   simp [option.is_none_iff_eq_none] at ha,
+    --   simp [ha, oracle_comp_base.reduce_pure],
+    -- }
   end }
-
--- instance is_lawful_monad (spec : oracle_spec) :
---   is_lawful_monad (oracle_comp spec) :=
--- { pure_bind := begin
---     intros α β a ob,
---     rw [bind_eq_thing],
---     rw [pure_eq_thing],
---     simp [quotient.lift_on_mk, oracle_comp_base.reduce],
---     obtain ⟨ob', h⟩ := quotient.exists_rep (ob a),
---     refine trans _ h,
---     refine quotient.sound _,
---     show oracle_comp_base.reduce _ = oracle_comp_base.reduce _,
---     refine trans (oracle_comp_base.reduce_pure_bind _ _) _,
---     rw [←h],
---     simp,
-
---   end,
---   bind_assoc := begin
---     intros α β γ oa ob oc,
---     -- by_cases h : β = γ,
---     simp only [bind_eq_thing],
---     obtain ⟨oa', h⟩ := quotient.exists_rep oa,
---     simp [← h],
---     -- refine quotient.sound _,
---     show oracle_comp_base.reduce _ = oracle_comp_base.reduce _,
---     simp [oracle_comp_base.reduce_bind_assoc],
---   -- simp [quotient.lift_on_mk, oracle_comp_base.reduce],
-
---   end,
---   id_map := begin
---     intros α oa,
---     show oa >>= (λ x, pure x) = oa,
---     rw [bind_eq_thing],
---     obtain ⟨oa', h⟩ := quotient.exists_rep oa,
---     simp [← h],
---     show oracle_comp_base.reduce _ = oracle_comp_base.reduce _,
---     induction oa' with α a α β oa ob hoa hob i t,
---     {
---       simp [oracle_comp_base.reduce, bind_eq_thing, pure_eq_thing],
---     },
---     {
---       simp [oracle_comp_base.reduce, bind_eq_thing, pure_eq_thing],
---       simp [oracle_comp_base.reduce_bind_pure],
---     },
---     {
---       rw [oracle_comp_base.reduce],
---       rw [oracle_comp_base.reduce],
-
---       simp [oracle_comp_base.reduce, bind_eq_thing, pure_eq_thing],
-
---     }
---     -- rw [pure_eq_thing],
---     -- simp [quotient.lift_on_mk, oracle_comp_base.reduce],
---   end
--- }
 
 end oracle_comp
